proofs/x86-64/avx2/ml_dsa_65/hashing.ec
@@ -1,0 +1,23 @@
+require import AllCore List (* IntDiv RealExp StdBigop *).
+
+from Jasmin require import JModel_x86.
+
+from JazzEC require import Ml_dsa_65_avx2 Mldsa_65_prelude Matrix_A Error_vectors T0 T1.
+(* from JazzEC require import Array32. *)
+
+from Spec require import GFq Rq Serialization Conversion Parameters VecMat
+                         Symmetric Sampling MLDSA_W32_Rep MLDSA.
+
+import PolyLVec PolyKVec PolyMat.
+import CDR Round Zq PolyReduceZq BigZMod.
+
+(* require import ArrayExtra JWord_extra EclibExtra JWordList. *)
+
+require import Array32 Array64 Array128 Array640 Array768 Array1280 Array1536 Array1920 Array1952 Array2496 Array4032 Array7680.
+require import WArray32 WArray1952 WArray4032.
+
+lemma hash_verification_key_correct _pk :
+    phoare [ M.hash_verification_key :
+         arg.`2 = _pk ==>
+         to_list res = Bytes64.to_list (H_tr (BytesPK.of_list (to_list _pk))) ] = 1%r.
+admitted.
