proofs/x86-64/avx2/ml_dsa_65/keygen.ec
@@ -1,0 +1,114 @@
+require import AllCore List (* IntDiv RealExp StdBigop *).
+
+from Jasmin require import JModel_x86.
+
+from JazzEC require import Ml_dsa_65_avx2 Mldsa_65_prelude Matrix_A Error_vectors T0 T1 S1 S2 Hashing.
+(* from JazzEC require import Array32. *)
+
+from Spec require import GFq Rq Serialization Conversion Parameters VecMat
+                         Symmetric Sampling MLDSA_W32_Rep MLDSA.
+
+import PolyLVec PolyKVec PolyMat.
+import CDR Round Zq PolyReduceZq BigZMod.
+
+(* require import ArrayExtra JWord_extra EclibExtra JWordList. *)
+
+require import Array32 Array64 Array128 Array256 Array320 Array640 Array768 Array1280 Array1536 Array1920 Array1952 Array2496 Array4032 Array7680.
+require import WArray32 WArray1952 WArray4032.
+
+require import Bindings.
+
+lemma keygen_internal
+    (RO <: LeakyRO):
+    equiv [ MLDSA(MLDSA_XOFA, MLDSA_XOFS, RO).keygen_derand ~ M.__keygen_internal :
+       Bytes32.to_list arg{1} = to_list arg{2}.`3
+     ==>
+       BytesPK.to_list res{1}.`2 = to_list res{2}.`1 /\
+       BytesSK.to_list res{1}.`1 = to_list res{2}.`2
+   ].
+proof.
+have Hkvec := mldsa65_kvec.
+proc => /=.
+seq 0 13 : #pre; 1: by auto.
+
+(* expanding seeds *)
+sp 2 0.
+seq 0 2 : (#pre /\
+ to_list prf_output{2} =
+   Bytes32.to_list rho{1} ++ Bytes64.to_list rhop{1} ++ Bytes32.to_list _K{1}).
++ admit. (* TODO: REFACTORING TO USE FORMOSA-KECCAK *)
+
+(* expanding A *)
+seq 1 2: (#pre /\ liftu_wpolymat (mat_unflatten256 matrix_A{2}) = _A{1} /\
+            wpolymat_urng (mat_unflatten256 matrix_A{2}) 1).
++ ecall{1} (ExpandA_correct rho{1}).
+  ecall{2} (matrix_A_correct seed_for_matrix_A{2}).
+  auto => /> &1 &2 _ _ H.
+  have Hn : forall i, 0 <= i < 128 => prf_output{2}.[i] =
+                     nth witness (Bytes32.to_list rho{1} ++ Bytes64.to_list rhop{1} ++ Bytes32.to_list _K{1}) i.
+  + by  move => kk kkb;rewrite -H  ?size_to_list 1:/#  !get_to_list.
+  move => rr -> ?;congr.
+  apply Bytes32.tP => k kb;rewrite Bytes32.get_of_list // get_to_list initiE 1:/# /=.  
+  by rewrite  Hn 1:/# -catA nth_cat ?Bytes32.size_to_list ifT 1:/#  Bytes32.get_to_list.
+
+(* expanding noise *)
+seq 0 2 : (#pre
+     /\ to_list seed_for_error_vectors{2} = Bytes64.to_list rhop{1}
+     /\ to_list seed_for_signing{2} = Bytes32.to_list _K{1}).
++ auto => /> &1 &2 _ _ H ?.
+  have Hn : forall i, 0 <= i < 128 => prf_output{2}.[i] =
+                     nth witness (Bytes32.to_list rho{1} ++ Bytes64.to_list rhop{1} ++ Bytes32.to_list _K{1}) i.
+  + by  move => kk kkb;rewrite -H  ?size_to_list 1:/#  !get_to_list.
+  split;apply (eq_from_nth witness);rewrite size_to_list ?Bytes32.size_to_list ?Bytes64.size_to_list //= => k kb; rewrite initiE 1:/# /= Hn 1:/# -catA nth_cat ?Bytes32.size_to_list ifF 1:/# nth_cat ?Bytes64.size_to_list.
+  + by rewrite ifT 1:/# Bytes64.get_to_list /#.
+  by rewrite ifF 1:/# Bytes32.get_to_list /#.
+
+seq 1 1 : (#pre
+     /\ lifts_wpolylvec (lvec_unflatten256 s1{2}) = s1{1}
+     /\ wpolylvec_srng (lvec_unflatten256 s1{2}) Eta Eta
+     /\ lifts_wpolykvec (kvec_unflatten256 s2{2}) = s2{1}
+     /\ wpolykvec_srng (kvec_unflatten256 s2{2}) Eta Eta).
++ ecall{1} (ExpandS_correct rhop{1}).
+  ecall{2} (error_vectors_correct seed_for_error_vectors{2}).
+  auto => /> &1 &2 _ _ _ _ ->.
+  by rewrite !Bytes64.to_listK => _ rr -> ? -> ?.
+
+proc change {2} [10..11] : [s1p : W32.t Array1280.t] {
+   s1p <@ M.row_vector__ntt(s1);
+   t <@ M.row_vector____multiply_with_matrix_A(matrix_A, s1p);
+}; 1: by sim.
+
+swap {2} [10..16] -9.
+
+seq 2 7 : (#pre
+      /\ lifts_wpolykvec (kvec_unflatten256 t0{2}) = t0{1}
+      /\ wpolykvec_srng (kvec_unflatten256 t0{2}) (dpow - 1) dpow 
+      /\ liftu_wpolykvec (kvec_unflatten256 t1{2}) = t1{1}
+      /\ wpolykvec_urng (kvec_unflatten256 t1{2}) b_t1
+ ); last first.
+
++ wp; ecall {2} (t0_encode_ph t0{2}).
+  wp; ecall {2} (hash_verification_key_correct verification_key_pointer_copy{2}).
+  wp; ecall {2} (t1_encode_ph t1{2}).
+  wp; ecall {2} (s2_encode_ph s2{2}).
+  wp; ecall {2} (s1_encode_ph s1{2}).
+
+  wp; ecall {1} (skEncode_corr rho{1} _K{1} tr{1} s1{1} s2{1} t0{1}).
+  wp; ecall {1} (pkEncode_corr rho{1} t1{1}).
+
+  auto => /> &1 &2 ?????????? rr1 Hrr11 rr2 Hrr21 Hrr22 rr3 Hrr31  rr4 Hrr41 Hrr42 rr5 Hrr5.
+  split.
+  + rewrite BytesPK.of_listK. 
+    + rewrite size_cat Bytes32.size_to_list (size_flatten_ctt 320).
+      + move =>x; rewrite mapP => He; elim He => xx /=.
+        rewrite /to_list mkseqP => [# He ->]; elim He => xxx /= => [# ??].
+        rewrite mapiE 1:/# initiE 1:/# /= => ->.
+        rewrite SimpleBitPack_liftE. admit.
+        by rewrite size_to_list.
+      by rewrite size_map /= size_to_list /#.
+    admit.
+  admit.
+
+admit.
+
+qed.
