proofs/x86-64/avx2/ml_dsa_65/sample/error_vectors.ec
@@ -1,0 +1,25 @@
+require import AllCore List (* IntDiv RealExp StdBigop *).
+
+from Jasmin require import JModel_x86.
+
+from JazzEC require import Ml_dsa_65_avx2 Mldsa_65_prelude.
+(* from JazzEC require import Array32. *)
+
+from Spec require import GFq Rq Serialization Conversion Parameters VecMat
+                         Symmetric Sampling MLDSA_W32_Rep MLDSA.
+
+import PolyLVec PolyKVec PolyMat.
+import CDR Round Zq PolyReduceZq BigZMod.
+
+(* require import ArrayExtra JWord_extra EclibExtra JWordList. *)
+
+require import Array32 Array64 Array128 Array256 Array1280 Array1952 Array4032 Array7680.
+
+phoare error_vectors_correct _rho :
+    [ M.sample____error_vectors : arg = _rho ==>
+        lifts_wpolylvec (lvec_unflatten256 res.`1) = (expandS (Bytes64.of_list (to_list _rho))).`1
+     /\ wpolylvec_srng (lvec_unflatten256 res.`1) Eta Eta
+     /\ lifts_wpolykvec (kvec_unflatten256 res.`2) = (expandS (Bytes64.of_list (to_list _rho))).`2
+     /\ wpolykvec_srng (kvec_unflatten256 res.`2) Eta Eta
+    ] = 1%r.
+admitted.
