proofs/x86-64/avx2/ml_dsa_65/sample/matrix_A.ec
@@ -1,0 +1,22 @@
+require import AllCore List (* IntDiv RealExp StdBigop *).
+
+from Jasmin require import JModel_x86.
+
+from JazzEC require import Ml_dsa_65_avx2 Mldsa_65_prelude.
+(* from JazzEC require import Array32. *)
+
+from Spec require import GFq Rq Serialization Conversion Parameters VecMat
+                         Symmetric Sampling MLDSA_W32_Rep MLDSA.
+
+import PolyLVec PolyKVec PolyMat.
+import CDR Round Zq PolyReduceZq BigZMod.
+
+(* require import ArrayExtra JWord_extra EclibExtra JWordList. *)
+
+require import Array32 Array128 Array256 Array1952 Array4032 Array7680.
+
+phoare matrix_A_correct _rho :
+    [ M.sample____matrix_A : arg = _rho ==>
+        liftu_wpolymat (mat_unflatten256 res) = expandA (Bytes32.of_list (to_list _rho))
+     /\ wpolymat_urng (mat_unflatten256 res) 1] = 1%r.
+admitted.
